fv/lean/Ragu/Circuits/Element/Mul.lean
@@ -9,56 +9,52 @@ structure Input (F : Type) where
   y : F
 deriving ProvableStruct
 
-def main (idx : ℕ) (input : Var Input (F p)) : Circuit (F p) (Var field (F p)) := do
-  let ⟨x, y, z⟩ ← (witness fun env => Core.AllocMul.readRow env.data idx
+def main (input : Var Input (F p)) : Circuit (F p) (Var field (F p)) := do
+  let ⟨x, y, z⟩ ← (witness fun env =>
+    let xv := Expression.eval env input.x
+    let yv := Expression.eval env input.y
+    ⟨xv, yv, xv * yv⟩
     : Circuit (F p) (Var Core.AllocMul.Row (F p)))
   assertZero (x * y - z)
   assertZero (x - input.x)
   assertZero (y - input.y)
   return z
 
-def Assumptions (idx : ℕ) (input : Input (F p)) (data : ProverData (F p)) :=
-  let w := Core.AllocMul.readRow data idx
-  w.x = input.x ∧ w.y = input.y ∧ w.x * w.y = w.z
+def Assumptions (_input : Input (F p)) (_data : ProverData (F p)) :=
+  True
 
 def Spec (input : Input (F p)) (out : field (F p)) (_data : ProverData (F p)) :=
   out = input.x * input.y
 
-instance elaborated (idx : ℕ) : ElaboratedCircuit (F p) Input field where
-  main := main idx
+instance elaborated : ElaboratedCircuit (F p) Input field where
+  main := main
   localLength _ := 3
 
-theorem soundness (idx : ℕ) : GeneralFormalCircuit.Soundness (F p) (elaborated idx) Spec := by
+theorem soundness : GeneralFormalCircuit.Soundness (F p) elaborated Spec := by
   circuit_proof_start
   obtain ⟨c1, c2, c3⟩ := h_holds
   rw [add_neg_eq_zero] at c1 c2 c3
   rw [←c2, ←c3, c1]
 
-theorem completeness (idx : ℕ) : GeneralFormalCircuit.Completeness (F p) (elaborated idx) (Assumptions idx) := by
+theorem completeness : GeneralFormalCircuit.Completeness (F p) elaborated Assumptions := by
   circuit_proof_start
   have h0 := h_env (0 : Fin 3)
   have h1 := h_env (1 : Fin 3)
   have h2 := h_env (2 : Fin 3)
-  simp only [toElements, circuit_norm, explicit_provable_type, Core.AllocMul.readRow, List.sum] at h0 h1 h2
+  simp only [toElements, circuit_norm, explicit_provable_type, Core.AllocMul.Row, List.sum] at h0 h1 h2
   norm_num at h0 h1 h2
   simp at h0 h1 h2
   rw [show i₀ + 1 + 1 = i₀ + 2 from by omega]
   rw [h0, h1, h2]
-  simp only [Core.AllocMul.readRow] at h_assumptions
-  obtain ⟨h_wx, h_wy, h_mul⟩ := h_assumptions
-  constructor
-  · rw [add_neg_eq_zero]; convert h_mul using 2 <;> simp
-  constructor
-  · rw [add_neg_eq_zero]; convert h_wx using 2 <;> simp
-  · rw [add_neg_eq_zero]; convert h_wy using 2 <;> simp
+  refine ⟨?_, ?_, ?_⟩ <;> ring
 
-def circuit (idx : ℕ) : GeneralFormalCircuit (F p) Input field :=
+def circuit : GeneralFormalCircuit (F p) Input field :=
   {
-    elaborated idx with
-    Assumptions := Assumptions idx,
+    elaborated with
+    Assumptions,
     Spec,
-    soundness := soundness idx,
-    completeness := completeness idx
+    soundness,
+    completeness
   }
 
 end Ragu.Circuits.Element.Mul
